feat(SMT): add HasType/RichHasType classes; retype lambda/forall binders
Replace the `vs_inj + vs_fresh` premises of the `lambda`/`forall` typing
rules with a single `vs_typed` premise driven by the new `HasType` class,
which assigns each variable an intrinsic SMT type. Add `RichHasType` for
typing determinism and the `Dom` instances in SMT.Semantics.

SMT/HOTyping/Rules.lean
@@ -6,7 +6,7 @@ section
 set_option hygiene false
 local notation:90 Γ:90 " ⊢ˢ' " x " : " τ:90 => Typing Γ x τ
 
-inductive Typing.{u} {𝒱 : Type u} [DecidableEq 𝒱] : TypeContext 𝒱 → Term 𝒱 → SMTType → Prop where
+inductive Typing.{u} {𝒱 : Type u} [DecidableEq 𝒱] [HasType 𝒱] : TypeContext 𝒱 → Term 𝒱 → SMTType → Prop where
   | var (Γ) (v τ) :
       Γ v = some τ
     ----------------
@@ -19,15 +19,13 @@ inductive Typing.{u} {𝒱 : Type u} [DecidableEq 𝒱] : TypeContext 𝒱 → T
     ------------------
     → Γ ⊢ˢ' .app f x : σ
   | lambda (Γ) {n} (τs : Fin n → SMTType) (t : (Fin n → 𝒱) → Term 𝒱) (γ) :
-      (∀ vs, (vs_inj : Function.Injective vs)
-        → (vs_fresh : ∀ i, (Γ (vs i)).isNone = true)
+      (∀ vs, (vs_typed : ∀ i, SMT.PHOAS.HasType.type (vs i) = τs i)
         → (Γ.update vs τs) ⊢ˢ' t vs : γ)
     → (n_pos : 0 < n)
     ------------------------------
     → Γ ⊢ˢ' .lambda τs t : .fun (Fin.foldr (n-1) (fun ⟨i, hi⟩ acc ↦ (τs ⟨i, Nat.lt_of_lt_pred hi⟩).pair acc) (τs ⟨n-1, Nat.sub_one_lt_of_lt n_pos⟩)) γ
   | forall (Γ) {n} (τs : Fin n → SMTType) (P : (Fin n → 𝒱) → Term 𝒱) :
-      (∀ vs, (vs_inj : Function.Injective vs)
-        → (vs_fresh : ∀ i, (Γ (vs i)).isNone = true)
+      (∀ vs, (vs_typed : ∀ i, SMT.PHOAS.HasType.type (vs i) = τs i)
         → (Γ.update vs τs) ⊢ˢ' P vs : .bool)
     → (n_pos : 0 < n)
     ------------------------------
@@ -124,38 +122,38 @@ notation:90 Γ:90 " ⊢ˢ' " x " : " τ:90 => Typing Γ x τ
 section InversionRules
 namespace Typing
 
-theorem varE      {𝒱} [DecidableEq 𝒱] {Γ : TypeContext 𝒱} {v τ} : Γ ⊢ˢ' .var v : τ → Γ v = .some τ := λ | var _ _ _ h => h
-theorem intE      {𝒱} [DecidableEq 𝒱] {Γ : TypeContext 𝒱} {n τ} : Γ ⊢ˢ' .int n : τ → τ = .int := λ | int _ _ => rfl
-theorem boolE     {𝒱} [DecidableEq 𝒱] {Γ : TypeContext 𝒱} {b τ} : Γ ⊢ˢ' .bool b : τ → τ = .bool := λ | bool _ _ => rfl
-theorem appE      {𝒱} [DecidableEq 𝒱] {Γ : TypeContext 𝒱} {f x σ} : Γ ⊢ˢ' .app f x : σ → ∃ τ, Γ ⊢ˢ' f : .fun τ σ ∧ Γ ⊢ˢ' x : τ := λ | app _ _ _ _ _ h₁ h₂ => ⟨_, h₁, h₂⟩
-theorem eqE       {𝒱} [DecidableEq 𝒱] {Γ : TypeContext 𝒱} {x y τ} : Γ ⊢ˢ' .eq x y : τ → τ = .bool ∧ ∃ σ, Γ ⊢ˢ' x : σ ∧ Γ ⊢ˢ' y : σ := λ | eq _ _ _ _ hx hy => ⟨rfl, _, hx, hy⟩
-theorem andE      {𝒱} [DecidableEq 𝒱] {Γ : TypeContext 𝒱} {x y τ} : Γ ⊢ˢ' .and x y : τ → τ = .bool ∧ Γ ⊢ˢ' x : .bool ∧ Γ ⊢ˢ' y : .bool := λ | and _ _ _ hx hy => ⟨rfl, hx, hy⟩
-theorem notE      {𝒱} [DecidableEq 𝒱] {Γ : TypeContext 𝒱} {x τ} : Γ ⊢ˢ' .not x : τ → τ = .bool ∧ Γ ⊢ˢ' x : .bool := λ | not _ _ h => ⟨rfl, h⟩
-theorem iteE      {𝒱} [DecidableEq 𝒱] {Γ : TypeContext 𝒱} {c t f τ} : Γ ⊢ˢ' .ite c t f : τ → Γ ⊢ˢ' c : .bool ∧ Γ ⊢ˢ' t : τ ∧ Γ ⊢ˢ' f : τ := λ | ite _ _ _ _ _ hc ht hf => ⟨hc,ht,hf⟩
-theorem someE     {𝒱} [DecidableEq 𝒱] {Γ : TypeContext 𝒱} {t τ} : Γ ⊢ˢ' .some t : τ → ∃ σ, τ = .option σ ∧ Γ ⊢ˢ' t : σ := λ | some _ _ _ h => ⟨_, rfl, h⟩
-theorem theE      {𝒱} [DecidableEq 𝒱] {Γ : TypeContext 𝒱} {t τ} : Γ ⊢ˢ' .the t : τ → Γ ⊢ˢ' t : τ.option := λ | the _ _ _ ht => ht
-theorem noneE     {𝒱} [DecidableEq 𝒱] {Γ : TypeContext 𝒱} {τ ξ} : Γ ⊢ˢ' .none ξ : τ → τ = .option ξ := λ | none .. => rfl
-theorem unitE     {𝒱} [DecidableEq 𝒱] {Γ : TypeContext 𝒱} {τ} : Γ ⊢ˢ' .«()» : τ → τ = .unit := λ | «()» .. => rfl
-theorem pairE     {𝒱} [DecidableEq 𝒱] {Γ : TypeContext 𝒱} {x y τ} : Γ ⊢ˢ' .pair x y : τ → ∃ α β, τ = .pair α β ∧ Γ ⊢ˢ' x : α ∧ Γ ⊢ˢ' y : β := λ | pair _ _ _ _ _ hx hy => ⟨_,_,rfl,hx,hy⟩
-theorem fstE      {𝒱} [DecidableEq 𝒱] {Γ : TypeContext 𝒱} {x τ} : Γ ⊢ˢ' .fst x : τ → ∃ σ, Γ ⊢ˢ' x : .pair τ σ := λ | fst _ _ _ _ hx => ⟨_,hx⟩
-theorem sndE      {𝒱} [DecidableEq 𝒱] {Γ : TypeContext 𝒱} {x τ} : Γ ⊢ˢ' .snd x : τ → ∃ σ, Γ ⊢ˢ' x : .pair σ τ := λ | snd _ _ _ _ hx => ⟨_,hx⟩
-theorem distinctE {𝒱} [DecidableEq 𝒱] {Γ : TypeContext 𝒱} {n : ℕ} {xs : Fin n → Term 𝒱} {τ} : Γ ⊢ˢ' .distinct xs : τ → τ = .bool ∧ ∃ σ, ∀ i, Γ ⊢ˢ' xs i : σ := λ | distinct _ _ σ h => ⟨rfl, σ, h⟩
-theorem leE       {𝒱} [DecidableEq 𝒱] {Γ : TypeContext 𝒱} {x y τ} : Γ ⊢ˢ' .le x y : τ → τ = .bool ∧ Γ ⊢ˢ' x : .int ∧ Γ ⊢ˢ' y : .int := λ | le _ _ _ hx hy => ⟨rfl,hx,hy⟩
-theorem addE      {𝒱} [DecidableEq 𝒱] {Γ : TypeContext 𝒱} {x y τ} : Γ ⊢ˢ' .add x y : τ → τ = .int ∧ Γ ⊢ˢ' x : .int ∧ Γ ⊢ˢ' y : .int := λ | add _ _ _ hx hy => ⟨rfl,hx,hy⟩
-theorem subE      {𝒱} [DecidableEq 𝒱] {Γ : TypeContext 𝒱} {x y τ} : Γ ⊢ˢ' .sub x y : τ → τ = .int ∧ Γ ⊢ˢ' x : .int ∧ Γ ⊢ˢ' y : .int := λ | sub _ _ _ hx hy => ⟨rfl,hx,hy⟩
-theorem mulE      {𝒱} [DecidableEq 𝒱] {Γ : TypeContext 𝒱} {x y τ} : Γ ⊢ˢ' .mul x y : τ → τ = .int ∧ Γ ⊢ˢ' x : .int ∧ Γ ⊢ˢ' y : .int := λ | mul _ _ _ hx hy => ⟨rfl,hx,hy⟩
-theorem lambdaE   {𝒱} [DecidableEq 𝒱] {Γ : TypeContext 𝒱} {n} {τs : Fin n → SMTType} {t : (Fin n → 𝒱) → Term 𝒱} {τ} : (h : Γ ⊢ˢ' .lambda τs t : τ) → 0 < n ∧ ∃ γ, τ = .fun (Fin.foldr (n-1) (fun ⟨i, hi⟩ acc ↦ (τs ⟨i, Nat.lt_of_lt_pred hi⟩).pair acc) (τs ⟨n-1, match h with | lambda _ _ _ _ _ h => Nat.sub_one_lt_of_lt h⟩)) γ ∧ (∀ vs, Function.Injective vs → (∀ i, (Γ (vs i)).isNone = true) → (Γ.update vs τs) ⊢ˢ' t vs : γ) := λ | .lambda _ _ _ γ typt n_pos => ⟨n_pos, γ, rfl, typt⟩
-theorem forallE   {𝒱} [DecidableEq 𝒱] {Γ : TypeContext 𝒱} {n} {τs : Fin n → SMTType} {P : (Fin n → 𝒱) → Term 𝒱} {τ} : Γ ⊢ˢ' .forall τs P : τ → 0 < n ∧ τ = .bool ∧ (∀ vs, Function.Injective vs → (∀ i, (Γ (vs i)).isNone = true) → (Γ.update vs τs) ⊢ˢ' P vs : .bool) := λ | .forall _ _ _ h n_pos => ⟨n_pos, rfl, h⟩
--- theorem orE       {𝒱} [DecidableEq 𝒱] {Γ : TypeContext 𝒱} {x y τ} : Γ ⊢ˢ' .or x y : τ → τ = .bool ∧ Γ ⊢ˢ' x : .bool ∧ Γ ⊢ˢ' y : .bool := λ | or _ _ _ hx hy => ⟨rfl, hx, hy⟩
--- theorem impE      {𝒱} [DecidableEq 𝒱] {Γ : TypeContext 𝒱} {x y τ} : Γ ⊢ˢ' .imp x y : τ → τ = .bool ∧ Γ ⊢ˢ' x : .bool ∧ Γ ⊢ˢ' y : .bool := λ | imp _ _ _ hx hy => ⟨rfl, hx, hy⟩
--- theorem existsE   {𝒱} [DecidableEq 𝒱] {Γ : TypeContext 𝒱} {n} {τs : Fin n → SMTType} {P : (Fin n → 𝒱) → Term 𝒱} {τ} : Γ ⊢ˢ' .exists τs P : τ → 0 < n ∧ τ = .bool ∧ (∀ vs, (Γ.update vs τs) ⊢ˢ' P vs : .bool) := λ | .exists _ _ _ h n_pos => ⟨n_pos, rfl, h⟩
+theorem varE      {𝒱} [DecidableEq 𝒱] [HasType 𝒱] {Γ : TypeContext 𝒱} {v τ} : Γ ⊢ˢ' .var v : τ → Γ v = .some τ := λ | var _ _ _ h => h
+theorem intE      {𝒱} [DecidableEq 𝒱] [HasType 𝒱] {Γ : TypeContext 𝒱} {n τ} : Γ ⊢ˢ' .int n : τ → τ = .int := λ | int _ _ => rfl
+theorem boolE     {𝒱} [DecidableEq 𝒱] [HasType 𝒱] {Γ : TypeContext 𝒱} {b τ} : Γ ⊢ˢ' .bool b : τ → τ = .bool := λ | bool _ _ => rfl
+theorem appE      {𝒱} [DecidableEq 𝒱] [HasType 𝒱] {Γ : TypeContext 𝒱} {f x σ} : Γ ⊢ˢ' .app f x : σ → ∃ τ, Γ ⊢ˢ' f : .fun τ σ ∧ Γ ⊢ˢ' x : τ := λ | app _ _ _ _ _ h₁ h₂ => ⟨_, h₁, h₂⟩
+theorem eqE       {𝒱} [DecidableEq 𝒱] [HasType 𝒱] {Γ : TypeContext 𝒱} {x y τ} : Γ ⊢ˢ' .eq x y : τ → τ = .bool ∧ ∃ σ, Γ ⊢ˢ' x : σ ∧ Γ ⊢ˢ' y : σ := λ | eq _ _ _ _ hx hy => ⟨rfl, _, hx, hy⟩
+theorem andE      {𝒱} [DecidableEq 𝒱] [HasType 𝒱] {Γ : TypeContext 𝒱} {x y τ} : Γ ⊢ˢ' .and x y : τ → τ = .bool ∧ Γ ⊢ˢ' x : .bool ∧ Γ ⊢ˢ' y : .bool := λ | and _ _ _ hx hy => ⟨rfl, hx, hy⟩
+theorem notE      {𝒱} [DecidableEq 𝒱] [HasType 𝒱] {Γ : TypeContext 𝒱} {x τ} : Γ ⊢ˢ' .not x : τ → τ = .bool ∧ Γ ⊢ˢ' x : .bool := λ | not _ _ h => ⟨rfl, h⟩
+theorem iteE      {𝒱} [DecidableEq 𝒱] [HasType 𝒱] {Γ : TypeContext 𝒱} {c t f τ} : Γ ⊢ˢ' .ite c t f : τ → Γ ⊢ˢ' c : .bool ∧ Γ ⊢ˢ' t : τ ∧ Γ ⊢ˢ' f : τ := λ | ite _ _ _ _ _ hc ht hf => ⟨hc,ht,hf⟩
+theorem someE     {𝒱} [DecidableEq 𝒱] [HasType 𝒱] {Γ : TypeContext 𝒱} {t τ} : Γ ⊢ˢ' .some t : τ → ∃ σ, τ = .option σ ∧ Γ ⊢ˢ' t : σ := λ | some _ _ _ h => ⟨_, rfl, h⟩
+theorem theE      {𝒱} [DecidableEq 𝒱] [HasType 𝒱] {Γ : TypeContext 𝒱} {t τ} : Γ ⊢ˢ' .the t : τ → Γ ⊢ˢ' t : τ.option := λ | the _ _ _ ht => ht
+theorem noneE     {𝒱} [DecidableEq 𝒱] [HasType 𝒱] {Γ : TypeContext 𝒱} {τ ξ} : Γ ⊢ˢ' .none ξ : τ → τ = .option ξ := λ | none .. => rfl
+theorem unitE     {𝒱} [DecidableEq 𝒱] [HasType 𝒱] {Γ : TypeContext 𝒱} {τ} : Γ ⊢ˢ' .«()» : τ → τ = .unit := λ | «()» .. => rfl
+theorem pairE     {𝒱} [DecidableEq 𝒱] [HasType 𝒱] {Γ : TypeContext 𝒱} {x y τ} : Γ ⊢ˢ' .pair x y : τ → ∃ α β, τ = .pair α β ∧ Γ ⊢ˢ' x : α ∧ Γ ⊢ˢ' y : β := λ | pair _ _ _ _ _ hx hy => ⟨_,_,rfl,hx,hy⟩
+theorem fstE      {𝒱} [DecidableEq 𝒱] [HasType 𝒱] {Γ : TypeContext 𝒱} {x τ} : Γ ⊢ˢ' .fst x : τ → ∃ σ, Γ ⊢ˢ' x : .pair τ σ := λ | fst _ _ _ _ hx => ⟨_,hx⟩
+theorem sndE      {𝒱} [DecidableEq 𝒱] [HasType 𝒱] {Γ : TypeContext 𝒱} {x τ} : Γ ⊢ˢ' .snd x : τ → ∃ σ, Γ ⊢ˢ' x : .pair σ τ := λ | snd _ _ _ _ hx => ⟨_,hx⟩
+theorem distinctE {𝒱} [DecidableEq 𝒱] [HasType 𝒱] {Γ : TypeContext 𝒱} {n : ℕ} {xs : Fin n → Term 𝒱} {τ} : Γ ⊢ˢ' .distinct xs : τ → τ = .bool ∧ ∃ σ, ∀ i, Γ ⊢ˢ' xs i : σ := λ | distinct _ _ σ h => ⟨rfl, σ, h⟩
+theorem leE       {𝒱} [DecidableEq 𝒱] [HasType 𝒱] {Γ : TypeContext 𝒱} {x y τ} : Γ ⊢ˢ' .le x y : τ → τ = .bool ∧ Γ ⊢ˢ' x : .int ∧ Γ ⊢ˢ' y : .int := λ | le _ _ _ hx hy => ⟨rfl,hx,hy⟩
+theorem addE      {𝒱} [DecidableEq 𝒱] [HasType 𝒱] {Γ : TypeContext 𝒱} {x y τ} : Γ ⊢ˢ' .add x y : τ → τ = .int ∧ Γ ⊢ˢ' x : .int ∧ Γ ⊢ˢ' y : .int := λ | add _ _ _ hx hy => ⟨rfl,hx,hy⟩
+theorem subE      {𝒱} [DecidableEq 𝒱] [HasType 𝒱] {Γ : TypeContext 𝒱} {x y τ} : Γ ⊢ˢ' .sub x y : τ → τ = .int ∧ Γ ⊢ˢ' x : .int ∧ Γ ⊢ˢ' y : .int := λ | sub _ _ _ hx hy => ⟨rfl,hx,hy⟩
+theorem mulE      {𝒱} [DecidableEq 𝒱] [HasType 𝒱] {Γ : TypeContext 𝒱} {x y τ} : Γ ⊢ˢ' .mul x y : τ → τ = .int ∧ Γ ⊢ˢ' x : .int ∧ Γ ⊢ˢ' y : .int := λ | mul _ _ _ hx hy => ⟨rfl,hx,hy⟩
+theorem lambdaE   {𝒱} [DecidableEq 𝒱] [HasType 𝒱] {Γ : TypeContext 𝒱} {n} {τs : Fin n → SMTType} {t : (Fin n → 𝒱) → Term 𝒱} {τ} : (h : Γ ⊢ˢ' .lambda τs t : τ) → 0 < n ∧ ∃ γ, τ = .fun (Fin.foldr (n-1) (fun ⟨i, hi⟩ acc ↦ (τs ⟨i, Nat.lt_of_lt_pred hi⟩).pair acc) (τs ⟨n-1, match h with | lambda _ _ _ _ _ h => Nat.sub_one_lt_of_lt h⟩)) γ ∧ (∀ vs, (∀ i, SMT.PHOAS.HasType.type (vs i) = τs i) → (Γ.update vs τs) ⊢ˢ' t vs : γ) := λ | .lambda _ _ _ γ typt n_pos => ⟨n_pos, γ, rfl, typt⟩
+theorem forallE   {𝒱} [DecidableEq 𝒱] [HasType 𝒱] {Γ : TypeContext 𝒱} {n} {τs : Fin n → SMTType} {P : (Fin n → 𝒱) → Term 𝒱} {τ} : Γ ⊢ˢ' .forall τs P : τ → 0 < n ∧ τ = .bool ∧ (∀ vs, (∀ i, SMT.PHOAS.HasType.type (vs i) = τs i) → (Γ.update vs τs) ⊢ˢ' P vs : .bool) := λ | .forall _ _ _ h n_pos => ⟨n_pos, rfl, h⟩
+-- theorem orE       {𝒱} [DecidableEq 𝒱] [HasType 𝒱] {Γ : TypeContext 𝒱} {x y τ} : Γ ⊢ˢ' .or x y : τ → τ = .bool ∧ Γ ⊢ˢ' x : .bool ∧ Γ ⊢ˢ' y : .bool := λ | or _ _ _ hx hy => ⟨rfl, hx, hy⟩
+-- theorem impE      {𝒱} [DecidableEq 𝒱] [HasType 𝒱] {Γ : TypeContext 𝒱} {x y τ} : Γ ⊢ˢ' .imp x y : τ → τ = .bool ∧ Γ ⊢ˢ' x : .bool ∧ Γ ⊢ˢ' y : .bool := λ | imp _ _ _ hx hy => ⟨rfl, hx, hy⟩
+-- theorem existsE   {𝒱} [DecidableEq 𝒱] [HasType 𝒱] {Γ : TypeContext 𝒱} {n} {τs : Fin n → SMTType} {P : (Fin n → 𝒱) → Term 𝒱} {τ} : Γ ⊢ˢ' .exists τs P : τ → 0 < n ∧ τ = .bool ∧ (∀ vs, (Γ.update vs τs) ⊢ˢ' P vs : .bool) := λ | .exists _ _ _ h n_pos => ⟨n_pos, rfl, h⟩
 
 end Typing
 end InversionRules
 
 instance {n} {𝒱} [Inhabited 𝒱] : Inhabited (Fin n → 𝒱) := inferInstance
 
-theorem Typing.det {𝒱} [DecidableEq 𝒱] [Inhabited 𝒱] {Γ : TypeContext 𝒱} {t : Term 𝒱} {τ σ : SMTType} :
+theorem Typing.det {𝒱} [DecidableEq 𝒱] [RichHasType 𝒱] [Inhabited 𝒱] {Γ : TypeContext 𝒱} {t : Term 𝒱} {τ σ : SMTType} :
     Γ ⊢ˢ' t : τ → Γ ⊢ˢ' t : σ → τ = σ := by
   intro typ_τ typ_σ
   induction t generalizing Γ τ σ with
@@ -248,10 +246,13 @@ theorem Typing.det {𝒱} [DecidableEq 𝒱] [Inhabited 𝒱] {Γ : TypeContext 
     obtain ⟨n_pos, γ, τ_eq, typ_t⟩ := Typing.lambdaE typ_τ
     obtain ⟨-, γ', σ_eq, typ_t'⟩ := Typing.lambdaE typ_σ
     rw [τ_eq, σ_eq]
-    -- typing under same Γ.update vs τs for any well-formed vs gives same γ
-    -- We need an injective fresh vs to specialize; this requires non-trivial structure.
-    -- For the of_abstract proof, we don't need det; leaving as sorry.
-    sorry
+    let vs : Fin _ → 𝒱 := fun i => RichHasType.rep (τs i)
+    have vs_typed : ∀ i, SMT.PHOAS.HasType.type (vs i) = τs i :=
+      fun i => RichHasType.rep_type (τs i)
+    have h1 := typ_t vs vs_typed
+    have h2 := typ_t' vs vs_typed
+    have := ih vs h1 h2
+    rw [this]
   | «forall» τs t ih =>
     obtain ⟨n_pos, rfl, typ_t⟩ := Typing.forallE typ_τ
     obtain ⟨-, rfl, typ_t'⟩ := Typing.forallE typ_σ
